src/impl/TLS13.Impl.ConnectionState.Queries.fst
@@ -6955,6 +6955,46 @@ fn read_negotiated_server_suite
   result
 }
 
+fn read_client_hello_kex_group
+  (c:connection_state)
+  (#st0:erased CS.connection_state)
+  requires connection_exactly c st0
+  returns g: CryptoSpec.kex_group
+  ensures connection_exactly c st0 **
+          pure (g == stored_client_hello_kex_group (Ghost.reveal st0))
+{
+  unfold (connection_exactly c st0);
+  unfold (connection_model_exactly c st0.CS.cs_model);
+  unfold (handshake_exactly c.handshake st0.CS.cs_model.CS.model_handshake);
+  unfold (handshake_messages_exactly
+    c.handshake.messages
+    st0.CS.cs_model.CS.model_handshake);
+  unfold (client_hello_metadata_exactly
+    c.handshake.messages.client_hello_has_server_name
+    c.handshake.messages.client_hello_server_name_len
+    c.handshake.messages.client_hello_cipher_suites_len
+    c.handshake.messages.client_hello_signature_schemes_len
+    c.handshake.messages.client_hello_session_id_len
+    c.handshake.messages.client_hello_kex_group
+    st0.CS.cs_model.CS.model_handshake.CS.hs_client_hello);
+  let g = !c.handshake.messages.client_hello_kex_group;
+  fold (client_hello_metadata_exactly
+    c.handshake.messages.client_hello_has_server_name
+    c.handshake.messages.client_hello_server_name_len
+    c.handshake.messages.client_hello_cipher_suites_len
+    c.handshake.messages.client_hello_signature_schemes_len
+    c.handshake.messages.client_hello_session_id_len
+    c.handshake.messages.client_hello_kex_group
+    st0.CS.cs_model.CS.model_handshake.CS.hs_client_hello);
+  fold (handshake_messages_exactly
+    c.handshake.messages
+    st0.CS.cs_model.CS.model_handshake);
+  fold (handshake_exactly c.handshake st0.CS.cs_model.CS.model_handshake);
+  fold (connection_model_exactly c st0.CS.cs_model);
+  fold (connection_exactly c st0);
+  g
+}
+
 fn read_client_hello_session_id
   (c:connection_state)
   (out:array U8.t)
